LeanYjs/ItemOriginOrder.lean
@@ -5,21 +5,15 @@ import Mathlib.Order.Defs.Unbundled
 open Relation
 
 variable (A : Type) [BEq A]
+inductive OriginLt : YjsPtr A -> YjsPtr A -> Prop where
+  | lt_left : forall o r id c, OriginLt o (YjsItem.item o r id c)
+  | lt_right : forall o r id c, OriginLt (YjsItem.item o r id c) r
+  | lt_first : forall item, OriginLt YjsPtr.first (YjsPtr.itemPtr item)
+  | lt_last : forall item, OriginLt (YjsPtr.itemPtr item) YjsPtr.last
+  | lt_first_last : OriginLt YjsPtr.first YjsPtr.last
 
-def IsItemClosed (P : YjsPtr A -> Prop) : Prop :=
-  P YjsPtr.first ∧
-  P YjsPtr.last ∧
-  (∀ (o : YjsPtr A) r id c, P (YjsItem.item o r id c) -> P o) ∧
-  (∀ o (r : YjsPtr A) id c, P (YjsItem.item o r id c) -> P r)
-
-def ClosedPredicate := { P : YjsPtr A -> Prop // IsItemClosed A P }
-
-inductive OriginLtStep : YjsPtr A -> YjsPtr A -> Prop where
-  | lt_left : forall o r id c, OriginLtStep o (YjsItem.item o r id c)
-  | lt_right : forall o r id c, OriginLtStep (YjsItem.item o r id c) r
-  | lt_first : forall item, OriginLtStep YjsPtr.first (YjsPtr.itemPtr item)
-  | lt_last : forall item, OriginLtStep (YjsPtr.itemPtr item) YjsPtr.last
-  | lt_first_last : OriginLtStep YjsPtr.first YjsPtr.last
+def OriginLeq (x y : YjsPtr A) : Prop :=
+  x = y ∨ OriginLt A x y
 
 inductive OriginReachableStep : YjsPtr A -> YjsPtr A -> Prop where
   | reachable : forall o r id c, OriginReachableStep (YjsItem.item o r id c) o
@@ -27,44 +21,23 @@ inductive OriginReachableStep : YjsPtr A -> YjsPtr A -> Prop where
 
 def OriginReachable := TransGen (r := @OriginReachableStep A)
 
-inductive OriginLt (P : @ClosedPredicate A): YjsPtr A -> YjsPtr A -> Prop where
-  | ltOrigin x y : P.val x -> P.val y -> OriginLtStep A x y -> OriginLt P x y
-  /-
-    if t is reachable, then t isn't between o and r
-    This means that (YjsItem.item o r id c) is neightbor of l and r at least when inserted.
-  -/
-  | ltReachableOrigin o r id c t :
-    P.val o -> P.val r -> P.val t ->
-    @OriginReachable A (YjsItem.item o r id c) t ->
-    OriginLt P t r ->
-    OriginLt P t o
-  | ltReachableRight o r id c t :
-    P.val o -> P.val r -> P.val t ->
-    @OriginReachable A (YjsItem.item o r id c) t ->
-    OriginLt P o t ->
-    OriginLt P r t
-  | ltTrans : forall x y z,
-    P.val x -> P.val y -> P.val z ->
-    OriginLt P x y -> OriginLt P y z -> OriginLt P x z
-
-lemma origin_lt_p1 {A} {P : @ClosedPredicate A} {x y : YjsPtr A} (h : OriginLt _ P x y) : P.val x := by
-  cases h with
-  | ltOrigin x y hpx hpy hlt =>
-    assumption
-  | ltReachableOrigin o r id c t ho hr ht hreach hlt =>
-    assumption
-  | ltReachableRight o r id c t ho hr ht hreach hlt =>
-    assumption
-  | ltTrans x y z hx hy hz hlt1 hlt2 =>
-    assumption
-
-lemma origin_lt_p2 {A} {P : @ClosedPredicate A} {x y : YjsPtr A} (h : OriginLt _ P x y) : P.val y := by
-  cases h with
-  | ltOrigin  y hpx hpy hlt
-    assumption
-  | ltReachableOrigin o r id c t ho hr ht hreach hlt =>
-    assumption
-  | ltReachableRight o r id c t ho hr ht hreach hlt =>
-    assumption
-  | ltTrans x y z hx hy hz hlt1 hlt2 =>
-    assumption
+-- inductive OriginLt (P : @ClosedPredicate A): YjsPtr A -> YjsPtr A -> Prop where
+--   | ltOrigin x y : P.val x -> P.val y -> OriginLtStep A x y -> OriginLt P x y
+--   /-
+--     if t is reachable, then t isn't between o and r
+--     This means that (YjsItem.item o r id c) is neightbor of l and r at least when inserted.
+--   -/
+--   -- | ltReachableOrigin o r id c t :
+--   --   P.val o -> P.val r -> P.val t ->
+--   --   @OriginReachable A (YjsItem.item o r id c) t ->
+--   --   OriginLt P t r ->
+--   --   OriginLt P t o
+--   -- | ltReachableRight o r id c t :
+--   --   P.val o -> P.val r -> P.val t ->
+--   --   @OriginReachable A (YjsItem.item o r id c) t ->
+--   --   OriginLt P o t ->
+--   --   OriginLt P r t
+--   | ltTrans : forall x y z,
+--     P.val x -> P.val y -> P.val z ->
+--     OriginReachable A x y -> OriginReachable A z y ->
+--     OriginLt P x y -> OriginLt P y z -> OriginLt P x z
