LeanYjs/ItemSetOrder.lean
@@ -1,0 +1,232 @@
+import LeanYjs.Item
+import LeanYjs.ItemSet
+import LeanYjs.ItemOriginOrder
+import LeanYjs.ActorId
+import LeanYjs.ItemOrder
+
+import Mathlib.Tactic.Set
+
+variable {A : Type} [BEq A]
+
+-- Defines a subset of YjsItem which are possible DAG of a history of insertions.
+
+variable (P : ClosedPredicate A)
+
+def YjsLt' (x y : YjsPtr A) : Prop :=
+  ∃ h, @YjsLt A P h x y
+
+def YjsLeq' (x y : YjsPtr A) : Prop :=
+  ∃ h, @YjsLeq A P h x y
+
+structure ItemSetInvariant where
+  origin_not_leq : ∀ (o r c id), P.val (YjsItem.item o r id c) -> ∀ h, ¬ YjsLeq P h r o
+  origin_nearest_reachable : ∀ (o r c id x),
+    P.val (YjsItem.item o r id c) ->
+    OriginReachable A (YjsItem.item o r id c) x ->
+    (∃ h, YjsLeq P h x o) ∨ (∃ h, YjsLeq P h r x)
+
+@[simp] lemma origin_p_valid {A} {P : ClosedPredicate A} : forall (x : YjsItem A), P.val x -> P.val x.origin := by
+  intros x px
+  obtain ⟨ p, ⟨ hp, hp', hp'', hp''' ⟩ ⟩ := P
+  simp at *
+  obtain ⟨ o, r, id, c ⟩ := x
+  simp [YjsItem.origin] at *
+  tauto
+
+@[simp] lemma right_origin_p_valid {A} {P : ClosedPredicate A} : forall (x : YjsItem A), P.val x -> P.val x.rightOrigin := by
+  intros x px
+  obtain ⟨ p, ⟨ hp, hp', hp'', hp''' ⟩ ⟩ := P
+  simp at *
+  obtain ⟨ o, r, id, c ⟩ := x
+  simp [YjsItem.rightOrigin] at *
+  tauto
+
+lemma not_item_lt_first {A} {P : ClosedPredicate A} : ItemSetInvariant P -> ∀ h (o : YjsItem A), ¬ @YjsLt A P h o YjsPtr.first := by
+  intros hinv h o
+  apply @Nat.strongRecOn' (P := fun h => ∀ (o : YjsItem A), ¬ @YjsLt A P h o YjsPtr.first)
+  intros n ih o hlt
+  cases hlt with
+  | ltConflict h _ _ hlt =>
+    cases hlt
+  | ltOriginOrder o _ po pf hlt =>
+    cases hlt with
+    | lt_right o' _ id  c =>
+      apply hinv.origin_not_leq _ _ _ _ po 0
+      cases o' with
+      | last =>
+        right
+        obtain ⟨ P, hP ⟩ := P
+        apply YjsLt.ltOriginOrder <;> try assumption
+        . apply hP.baseLast
+        . apply OriginLt.lt_first_last
+      | first =>
+        left
+        simp
+      | itemPtr item =>
+        right
+        obtain ⟨ P, hP ⟩ := P
+        apply YjsLt.ltOriginOrder <;> try assumption
+        . simp at *
+          apply hP.closedLeft; assumption
+        . apply OriginLt.lt_first
+  | ltTrans h1 h2 x y z hlt1 hlt2 =>
+    have hlt_h2 : h2 < max h1 h2 + 1 := by
+      omega
+    apply ih _ hlt_h2 _ hlt2
+
+lemma not_last_lt_item {A} {P : ClosedPredicate A} : ItemSetInvariant P -> ∀ h (o : YjsItem A), ¬ @YjsLt A P h YjsPtr.last o := by
+  intros hinv h o
+  apply @Nat.strongRecOn' (P := fun h => ∀ (o : YjsItem A), ¬ @YjsLt A P h YjsPtr.last o)
+  intros n ih o hlt
+  cases hlt with
+  | ltConflict h _ _ hlt =>
+    cases hlt
+  | ltOriginOrder _ _ _ hpo hlt =>
+    have hlt2 : @OriginLt A o YjsPtr.last := by
+      apply OriginLt.lt_last
+    cases hlt with
+    | lt_left o' r id c =>
+      apply hinv.origin_not_leq _ _ _ _ hpo 0
+      cases r with
+      | last =>
+        left
+        simp
+      | first =>
+        right
+        obtain ⟨ P, hP ⟩ := P
+        apply YjsLt.ltOriginOrder <;> try assumption
+        . apply hP.baseFirst
+        . apply OriginLt.lt_first_last
+      | itemPtr item =>
+        right
+        obtain ⟨ P, hP ⟩ := P
+        apply YjsLt.ltOriginOrder <;> try assumption
+        . simp at *
+          apply hP.closedRight; assumption
+        . apply OriginLt.lt_last
+  | ltTrans h1 h2 x y z hlt1 hlt2 =>
+    have hlt_h2 : h1 < max h1 h2 + 1 := by
+      omega
+    apply ih _ hlt_h2 _ hlt1
+
+lemma not_last_lt_first {A} {P : ClosedPredicate A} : ItemSetInvariant P -> ∀ h, ¬ @YjsLt A P h YjsPtr.last YjsPtr.first := by
+  intros hinv h
+  apply @Nat.strongRecOn' (P := fun h => ¬ @YjsLt A P h YjsPtr.last YjsPtr.first)
+  intros n ih hlt
+  cases hlt with
+  | ltConflict h _ _ hlt =>
+    cases hlt
+  | ltOriginOrder _ _ _ _ hlt =>
+    cases hlt
+  | ltTrans h1 h2 x y z hlt1 hlt2 =>
+    apply not_item_lt_first at hlt2 <;> assumption
+
+lemma not_first_lt_first {A} {P : ClosedPredicate A} : ItemSetInvariant P -> ∀ h, ¬ @YjsLt A P h YjsPtr.first YjsPtr.first := by
+  intros hinv h hlt
+  have h: OriginLt A YjsPtr.first YjsPtr.first := by
+    cases hlt with
+    | ltConflict h _ _ hlt =>
+      cases hlt
+    | ltTrans h1 h2 x y z hlt1 hlt2 =>
+      apply not_item_lt_first hinv at hlt2; contradiction
+    | ltOriginOrder _ _ hlt =>
+      assumption
+  cases h with
+
+lemma not_last_lt_last {A} {P : ClosedPredicate A} : ItemSetInvariant P -> ∀ h, ¬ @YjsLt A P h YjsPtr.last YjsPtr.last := by
+  intros hinv h hlt
+  have h: OriginLt A YjsPtr.last YjsPtr.last := by
+    cases hlt with
+    | ltConflict h _ _ hlt =>
+      cases hlt
+    | ltTrans h1 h2 x y z hlt1 hlt2 =>
+      apply not_last_lt_item hinv at hlt1; contradiction
+    | ltOriginOrder _ _ hlt =>
+      assumption
+  cases h with
+
+lemma not_ptr_lt_first {A} {P : ClosedPredicate A} : ItemSetInvariant P -> ∀ h (o : YjsPtr A), ¬ @YjsLt A P h o YjsPtr.first := by
+  intros hinv h o
+  cases o with
+  | itemPtr item =>
+    apply not_item_lt_first hinv
+  | first =>
+    apply not_first_lt_first hinv
+  | last =>
+    apply not_last_lt_first hinv
+
+lemma not_last_lt_ptr {A} {P : ClosedPredicate A} : ItemSetInvariant P -> ∀ h (o : YjsPtr A), ¬ @YjsLt A P h YjsPtr.last o := by
+  intros hinv h o
+  cases o with
+  | itemPtr item =>
+    apply not_last_lt_item hinv
+  | first =>
+    apply not_last_lt_first hinv
+  | last =>
+    apply not_last_lt_last hinv
+
+lemma yjs_lt_p_trans {A} {P : ClosedPredicate A} (inv : ItemSetInvariant P) (x y z : YjsPtr A) h1 h2:
+  @YjsLt A P h1 x y -> @YjsLt A P h2 y z -> @YjsLt A P (max h1 h2 + 1) x z := by
+  intros hlt1 hlt2
+  cases y with
+  | first =>
+    apply not_ptr_lt_first inv at hlt1; contradiction
+  | last =>
+    apply not_last_lt_ptr inv at hlt2; contradiction
+  | itemPtr y =>
+    apply YjsLt.ltTrans <;> assumption
+
+lemma yjs_leq_p_trans1 {A} {P : ClosedPredicate A} (inv : ItemSetInvariant P) (x y z : YjsPtr A) h1 h2:
+  @YjsLeq A P h1 x y -> @YjsLt A P h2 y z -> ∃ h, @YjsLt A P h x z := by
+  intros hleq hlt
+  cases hleq with
+  | inl heq =>
+    rw [heq]
+    exists h2
+  | inr hlt =>
+    exists (max h1 h2 + 1)
+    apply yjs_lt_p_trans <;> assumption
+
+lemma yjs_leq_p_trans2 {A} {P : ClosedPredicate A} (inv : ItemSetInvariant P) (x y z : YjsPtr A) h1 h2:
+  @YjsLt A P h1 x y -> @YjsLeq A P h2 y z -> ∃ h, @YjsLt A P h x z := by
+  intros hlt hleq
+  cases hleq with
+  | inl heq =>
+    rw [<-heq]
+    exists h1
+  | inr hlt =>
+    exists (max h1 h2 + 1)
+    apply yjs_lt_p_trans <;> assumption
+
+lemma yjs_leq_p_trans {A} {P : ClosedPredicate A} (inv : ItemSetInvariant P) (x y z : YjsPtr A) h1 h2:
+  @YjsLeq A P h1 x y -> @YjsLeq A P h2 y z -> ∃ h, @YjsLeq A P h x z := by
+  intros hleq1 hleq2
+  cases hleq1 with
+  | inl heq =>
+    rw [heq]
+    exists h2
+  | inr hlt =>
+    cases hleq2 with
+    | inl heq =>
+      rw [<-heq]
+      exists h1
+      right
+      assumption
+    | inr hlt =>
+      exists (max h1 h2 + 1)
+      right
+      apply yjs_lt_p_trans <;> assumption
+
+-- lemma origin_lt_p1 {A} {P : @ClosedPredicate A} {x y : YjsPtr A} (h : OriginLt _ x y) : P.val x := by
+--   sorry
+
+-- lemma origin_lt_p2 {A} {P : @ClosedPredicate A} {x y : YjsPtr A} (h : OriginLt _ x y) : P.val y := by
+--   cases h with
+--   | ltOrigin  y hpx hpy hlt
+--     assumption
+--   -- | ltReachableOrigin o r id c t ho hr ht hreach hlt =>
+--   --   assumption
+--   -- | ltReachableRight o r id c t ho hr ht hreach hlt =>
+--   --   assumption
+--   | ltTrans x y z hx hy hz hlt1 hlt2 =>
+--     assumption
